platform/cito/GLabelMapFacts.v
@@ -1,0 +1,14 @@
+Set Implicit Arguments.
+
+Require Import GLabelKey.
+Module K := GLabel_as_UDT.
+Require Import GLabelMap.
+Module M := GLabelMap.
+Require Import FMapFacts.
+Include (Properties M).
+Include (Facts M).
+Require Import FMapFacts1.
+Include (WFacts_fun K M).
+Include (UWFacts_fun K M).
+Require Import FMapFacts2.
+Include (UWFacts_fun K M).
